Cslib/Languages/LambdaCalculus/LocallyNameless/Untyped/Properties.lean
@@ -116,6 +116,10 @@ theorem beta_lc {M N : Term Var} (m_lc : M.abs.LC) (n_lc : LC N) : LC (M ^ N) :=
   cases m_lc with
   | abs => grind [fresh_exists <| free_union [fv] Var]
 
+@[scoped grind ←]
+theorem beta_lc_reverse {M N : Term Var} (m_lc : M.abs.LC) (n_lc : LC N) : LC (M ^ N) := by
+
+
 /-- Opening then closing is equivalent to substitution. -/
 @[scoped grind =]
 lemma open_close_to_subst (m : Term Var) (x y : Var) (k : ℕ) (m_lc : LC m) :
